add definition of typing rule

CSL.v
@@ -5,7 +5,6 @@ Require Import ZArith.
 Require Import String.
 Require Import QArith.
 Require Import Qcanon.
-
 Require Import Coq.Relations.Relations.
 
 Require ClassicalFacts.
@@ -23,22 +22,22 @@ Set Implicit Arguments.
 Unset Strict Implicit.
 
 Module PHeap.
-  Definition pheap := Z -> option (Qc * Z).
+  Definition pheap' := Z -> option (Qc * Z).
 
-  Definition is_pheap (h : pheap) : Prop :=
+  Definition is_pheap (h : pheap') : Prop :=
     forall x, match h x with
       | None => True
       | Some (p, v) => 0 < p /\ p <= 1
     end.
-  
-  Definition pdisj (h1 h2 : pheap) :=
+  Record pheap := Pheap { this :> pheap'; is_p : is_pheap this }.
+  Definition pdisj (h1 h2 : pheap') :=
     forall (x : Z), match h1 x, h2 x with
       | None, _ | _, None => True
       | Some (p1, v1), some (p2, v2) =>
         v1 = v2 /\ 0 < p1 + p2 /\ p1 + p2 <= 1
     end.
 
-  Definition phplus (h1 h2 : pheap) : pheap :=
+  Definition phplus (h1 h2 : pheap') : pheap' :=
     fun x => match h1 x with
      | None => h2 x
      | Some (p1, v1) => 
@@ -49,9 +48,9 @@ Module PHeap.
      end.
 
   Definition full_p : Qc := 1.
-  Definition emp_h : pheap := fun (n : Z) => None.
+  Definition emp_h : pheap' := fun (n : Z) => None.
 
-  Definition fpdom (h : pheap) : Prop :=
+  Definition fpdom (h : pheap') : Prop :=
     forall (n : Z), match h n with
       | None => True
       | Some (p, v) => (p = full_p)%Qc
@@ -59,7 +58,7 @@ Module PHeap.
   
   Lemma pdisjC : forall h1 h2, pdisj h1 h2 -> pdisj h2 h1.
   Proof. 
-    unfold pdisj, pheap; intros h1 h2 hd x.
+    unfold pdisj, pheap'; intros h1 h2 hd x.
     specialize (hd x).
     destruct (h1 x), (h2 x); try tauto.
     destruct p as [? ?], p0 as [? ?].
@@ -72,11 +71,11 @@ Module PHeap.
   Qed.
 
   Lemma pdisj_empty2 : forall (h : pheap), pdisj h emp_h.
-    now unfold emp_h, pdisj; simpl; intros h x; destruct (h x) as [[? ?] | ?].
+     now unfold emp_h, pdisj; intros h x; destruct (this h x) as [[? ?] | ?].
   Qed.
 
-  Definition ph_upd (h : pheap) (x : Z) (v : Z) : pheap :=
-    fun (x' : Z) => if Zeq_bool x x' then Some (full_p, v) else h x'.
+  Definition ph_upd (h : pheap') (x : Z) (v : Z) : pheap' :=
+    fun (x' : Z) => if Z.eq_dec x x' then Some (full_p, v) else h x'.
 
   Definition empty_p := 0.
 
@@ -97,26 +96,26 @@ Module PHeap.
     auto using frac_contra1.
   Qed.
   
-  Lemma pdisj_upd : forall (h h' : pheap) (H : is_pheap h) (H' : is_pheap h')
-    (x w v : Z), h x = Some (full_p, w) -> 
+  Lemma pdisj_upd : forall (h h' : pheap) (x w v : Z), this h x = Some (full_p, w) -> 
     (pdisj (ph_upd h x v) h' <-> pdisj h h').
   Proof.
+    destruct h as [h iph].
+    destruct h' as [h' iph'].
     unfold pdisj, ph_upd; ins.
     split. 
-    - intros hp x0; specialize (hp x0); specialize (H x0); specialize (H' x0).
-      destruct (Zeq_bool x x0), (h x0) as [[? ?] | ], (h' x0) as [[? ?] | ]; eauto.
-      destruct hp as [? [? ?]],  H' as [? ?]; exfalso; eapply (@frac_contra1 q0); eauto.
-    - intros hp x0; specialize (hp x0); specialize (H x0); specialize (H' x0).
-      pose proof (Zeq_bool_if x x0); 
-      destruct (Zeq_bool x x0); subst;
+    - intros hp x0; pose proof (hp x0); pose proof (iph x0); pose proof (iph' x0).
+      destruct (Z.eq_dec x x0), (h x0) as [[? ?] | ], (h' x0) as [[? ?] | ]; eauto.
+      destruct H0 as [? [? ?]],  H2 as [? ?]; exfalso; eapply (@frac_contra1 q0); eauto.
+    - intros hp x0; specialize (hp x0); specialize (iph x0); specialize (iph' x0).
+      destruct (Z.eq_dec x x0); subst;
       destruct (h x0) as [[? ?] | ], (h' x0) as [[? ?] | ]; simpl; eauto;
-      inversion H0; subst.
-      destruct hp as [? [? ?]], H' as [? ?]; exfalso; eapply (@frac_contra1 q0); eauto.
+      inversion H; subst.
+      destruct hp as [? [? ?]], iph' as [? ?]; exfalso; eapply (@frac_contra1 q0); eauto.
   Qed.
 
-  Lemma phplus_comm (h1 h2 : pheap) (H1 : is_pheap h1) (H2 : is_pheap h2) :
-    pdisj h1 h2 -> phplus h1 h2 = phplus h2 h1.
+  Lemma phplus_comm (h1 h2 : pheap) : pdisj h1 h2 -> phplus h1 h2 = phplus h2 h1.
   Proof.
+    destruct h1 as [h1 H1], h2 as [h2 H2]; simpl.
     intros hdisj; unfold is_pheap, pdisj, phplus in *; extensionality x.
     repeat (match goal with [H : forall _ : Z, _ |- _] => specialize (H x) end).
     destruct (h1 x) as [[? ?] | ], (h2 x) as [[? ?] | ]; eauto. 
@@ -147,26 +146,27 @@ Module PHeap.
     apply (Qclt_le_trans _ (p + p1) _); [apply gt_0_plus; eauto | eauto].
   Qed.
 
-  Lemma pdisj_padd (h1 h2 h3 : pheap) (ph1 : is_pheap h1) (ph2 : is_pheap h2) (ph3 : is_pheap h3) :
+  Lemma pdisj_padd (h1 h2 h3 : pheap) :
     pdisj h2 h3 -> pdisj h1 (phplus h2 h3) -> (pdisj h1 h2) /\ (pdisj h1 h3).
   Proof.
+    destruct h1 as [h1 H1], h2 as [h2 H2], h3 as [h3 H3]; simpl.
     unfold is_pheap, pdisj, phplus in *;
     intros disj23 disj123; split; intros x; 
     repeat (match goal with [H : forall _ : Z, _ |- _] => specialize (H x) end);
     destruct (h1 x) as [[? ?] |], (h2 x) as [[? ?] |], (h3 x) as [[? ?] |];
-    destruct disj23 as [? [? ?]], disj123 as [? [? ?]], ph1 as [? ?], ph2 as [? ?], ph3 as [? ?];
+    destruct disj23 as [? [? ?]], disj123 as [? [? ?]], H1 as [? ?], H2 as [? ?], H3 as [? ?];
     repeat split; eauto using Qcplus_comm.
 
     - apply plus_gt_0; eauto.
-    - cutrewrite (q + (q0 + q1) = (q + q0) + q1) in H4; [apply (@le1_weak _ q1); eauto | ring ].
+    - cutrewrite (q + (q0 + q1) = (q + q0) + q1) in H7; [apply (@le1_weak _ q1); eauto | ring ].
     - congruence.
     - apply plus_gt_0; eauto.
-    - cutrewrite (q + (q0 + q1) = (q + q1) + q0) in H4; [apply (@le1_weak _ q0); eauto | ring ].
+    - cutrewrite (q + (q0 + q1) = (q + q1) + q0) in H7; [apply (@le1_weak _ q0); eauto | ring ].
   Qed.
 
-  Lemma pdisjE1 (h1 h2 h3 : pheap) (ph1 : is_pheap h1) (ph2 : is_pheap h2) (ph3 : is_pheap h3) :
-    pdisj h1 (phplus h2 h3) -> pdisj h2 h3 -> pdisj h1 h2.
+  Lemma pdisjE1 (h1 h2 h3 : pheap) : pdisj h1 (phplus h2 h3) -> pdisj h2 h3 -> pdisj h1 h2.
   Proof.
+    destruct h1 as [h1 ph1], h2 as [h2 ph2], h3 as [h3 ph3]; simpl in *.
     unfold is_pheap, pdisj, phplus in *;
     intros h123 h23 x;
     repeat (match goal with [H : forall _ : Z, _ |- _] => specialize (H x) end).
@@ -176,9 +176,10 @@ Module PHeap.
     cutrewrite (q + (q0 + q1) = (q + q0) + q1) in H7; [apply (@le1_weak _ q1); eauto | ring ].
   Qed.
 
-  Lemma pdisjE2 (h1 h2 h3 : pheap) (ph1 : is_pheap h1) (ph2 : is_pheap h2) (ph3 : is_pheap h3) :
+  Lemma pdisjE2 (h1 h2 h3 : pheap) :
     pdisj h1 (phplus h2 h3) -> pdisj h2 h3 -> pdisj h1 h3.
   Proof.
+    destruct h1 as [h1 ph1], h2 as [h2 ph2], h3 as [h3 ph3]; simpl in *.
     unfold is_pheap, pdisj, phplus in *;
     intros h123 h23 x;
     repeat (match goal with [H : forall _ : Z, _ |- _] => specialize (H x) end).
@@ -189,9 +190,10 @@ Module PHeap.
     - cutrewrite (q + (q0 + q1) = (q + q1) + q0) in H7; [apply (@le1_weak _ q0); eauto | ring ].
   Qed.
 
-  Lemma pdisj_padd_comm (h1 h2 h3 : pheap) (ph1 : is_pheap h1) (ph2 : is_pheap h2) (ph3 : is_pheap h3) :
-    pdisj h2 (phplus h1 h3) -> pdisj h1 h3 -> pdisj h1 (phplus h2 h3).
+  Lemma pdisj_padd_comm (h1 h2 h3 : pheap) : pdisj h2 (phplus h1 h3) -> pdisj h1 h3 -> 
+                                             pdisj h1 (phplus h2 h3).
   Proof.
+    destruct h1 as [h1 ph1], h2 as [h2 ph2], h3 as [h3 ph3]; simpl in *.
     unfold is_pheap, pdisj, phplus in *;
     intros h123 h23 x;
     repeat (match goal with [H : forall _ : Z, _ |- _] => specialize (H x) end).
@@ -204,9 +206,10 @@ Module PHeap.
   Qed.
 
   Lemma pdisj_padd_expand 
-        (h1 h2 h3 : pheap) (ph1 : is_pheap h1) (ph2 : is_pheap h2) (ph3 : is_pheap h3) :
-    pdisj h1 h2 -> (pdisj (phplus h1 h2) h3 <-> (pdisj h1 (phplus h2 h3) /\ pdisj h2 h3)).
+        (h1 h2 h3 : pheap) : pdisj h1 h2 -> 
+                             (pdisj (phplus h1 h2) h3 <-> (pdisj h1 (phplus h2 h3) /\ pdisj h2 h3)).
   Proof.
+    destruct h1 as [h1 ph1], h2 as [h2 ph2], h3 as [h3 ph3]; simpl in *.
     unfold is_pheap, pdisj, phplus in *;
     intros h12; split; [intros H; split; intros x | intros [H1 H2] x];
     repeat (match goal with [H : forall _ : Z, _ |- _] => specialize (H x) end);
@@ -222,9 +225,10 @@ Module PHeap.
   Qed.
 
   Lemma padd_assoc
-        (h1 h2 h3 : pheap) (ph1 : is_pheap h1) (ph2 : is_pheap h2) (ph3 : is_pheap h3) :
+        (h1 h2 h3 : pheap)  :
     pdisj h1 (phplus h2 h3) -> pdisj h2 h3 -> phplus (phplus h1 h2) h3 = phplus h1 (phplus h2 h3).
   Proof.
+    destruct h1 as [h1 ph1], h2 as [h2 ph2], h3 as [h3 ph3]; simpl in *.
     unfold is_pheap, pdisj, phplus in *;
     intros h123 h23; extensionality x;
     repeat (match goal with [H : forall _ : Z, _ |- _] => specialize (H x) end);
@@ -234,9 +238,10 @@ Module PHeap.
   Qed.
 
   Lemma padd_left_comm 
-        (h1 h2 h3 : pheap) (ph1 : is_pheap h1) (ph2 : is_pheap h2) (ph3 : is_pheap h3) :
+        (h1 h2 h3 : pheap) :
     pdisj h1 (phplus h2 h3) -> pdisj h2 h3 -> phplus h1 (phplus h2 h3) = phplus h2 (phplus h1 h3).
   Proof.
+    destruct h1 as [h1 ph1], h2 as [h2 ph2], h3 as [h3 ph3]; simpl in *.
     unfold is_pheap, pdisj, phplus in *;
     intros h123 h23; extensionality x;
     repeat (match goal with [H : forall _ : Z, _ |- _] => specialize (H x) end);
@@ -247,10 +252,14 @@ Module PHeap.
   Qed.
   
   Lemma padd_cancel
-        (h1 h2 h3 : pheap) (ph1 : is_pheap h1) (ph2 : is_pheap h2) (ph3 : is_pheap h3) :
+        (h1 h2 h3 : pheap) :
     phplus h1 h2 = phplus h1 h3 -> pdisj h1 h2 -> pdisj h1 h3 -> h2 = h3.
+  Proof.
+    destruct h1 as [h1 ph1], h2 as [h2 ph2], h3 as [h3 ph3]; simpl in *.
+    intros heq h12 h13.
+    assert (h2 = h3).
     unfold is_pheap, pdisj, phplus in *;
-    intros heq h12 h13; extensionality x; pose proof  (equal_f heq x) as heq'; simpl in *; clear heq;
+    extensionality x; pose proof  (equal_f heq x) as heq'; simpl in *; clear heq;
     repeat (match goal with [H : forall _ : Z, _ |- _] => specialize (H x) end);
     destruct (h1 x) as [[? ?] |], (h2 x) as [[? ?] |], (h3 x) as [[? ?] |];
     des; eauto; try congruence.
@@ -272,19 +281,30 @@ Module PHeap.
       cutrewrite (q - q = 0) in H; [| ring].
       cutrewrite (q + q0 - q = q0) in H; [| ring].
       rewrite <- H in ph3; inversion ph3.
+    - subst; cutrewrite (ph2 = ph3); [eauto | apply proof_irrelevance ].
   Qed.
-  
-  Definition ptoheap (ph : pheap) (h : heap) : Prop :=
+
+  Corollary padd_cancel2 (h1 h2 h3 : pheap) :
+    phplus h2 h1 = phplus h3 h1 -> pdisj h2 h1 -> pdisj h3 h1 -> h2 = h3.
+  Proof.
+    Hint Resolve pdisjC.
+    intros.
+    rewrite (@phplus_comm h2 h1), (@phplus_comm h3 h1) in H; eauto.
+    eapply padd_cancel; eauto.
+  Qed.
+
+  Definition ptoheap (ph : pheap') (h : heap) : Prop :=
     forall (x : Z), match ph x with
       | None => h x = None
       | Some (p, v) => p = full_p /\ h x = Some v
     end.
 
-  Lemma ptoD (ph1 ph2 : pheap) (h : heap) (hp1 : is_pheap ph1) (hp2 : is_pheap ph2) :
+  Lemma ptoD (ph1 ph2 : pheap') (h : heap):
     ptoheap ph1 h -> ptoheap ph2 h -> ph1 = ph2.
   Proof.
-    unfold is_pheap, pdisj, phplus, ptoheap in *;
-    intros pto1 pto2; extensionality x;
+(*    destruct ph1 as [h1 ph1], ph2 as [h2 ph2]; simpl in *.*)
+    intros pto1 pto2.
+    unfold is_pheap, pdisj, phplus, ptoheap in *; extensionality x; simpl in *;
     repeat (match goal with [H : forall _ : Z, _ |- _] => specialize (H x) end);
     destruct (ph1 x) as [[? ?] |], (ph2 x) as [[? ?] |];
     des; eauto; try congruence.
@@ -386,56 +406,42 @@ Module Language.
   
   Notation "c '/' st  '==>s*'  c' '/' st' " := (multi_red c st c' st') (at level 40, st at level 39, c' at level 39).
 
-  Definition pstate := (stack * pheap)%type.
-  
-  Inductive red_p: (cmd * pstate) -> (cmd * pstate) -> Prop :=
-    redp_ster : forall (c1 c2 : cmd) (st1 st2 : stack) (ph1 ph2 phF : pheap) (h1 h2 : heap),
-      is_pheap ph1 -> is_pheap ph2 -> is_pheap phF ->
-      pdisj ph1 phF -> ptoheap (phplus ph1 phF) h1 ->
-      c1 / (st1, h1) ==>s c2 / (st2, h2) ->
-      pdisj ph2 phF -> ptoheap (phplus ph2 phF) h2 ->
-      red_p (c1, (st1, ph1)) (c2, (st2, ph2)).
-  Notation "c '/' st  '==>p'  c' '/' st' " := (red_p (c, st) (c', st')) (at level 40, st at level 39, c' at level 39).
-
-  Lemma red_det (st st1 st2 : (cmd * state)) :
-    fst st / snd st ==>s fst st1 / snd st1 -> 
-    fst st / snd st ==>s fst st2 / snd st2 -> 
-    fst st1 = fst st2 /\ snd st1 = snd st2.
+  Lemma red_det (c c1 c2 : cmd) (st st1 st2 : state) :
+    c / st ==>s c1 / st1 ->
+    c / st ==>s c2 / st2 ->
+    c1 = c2 /\ st1 = st2.
   Proof.
     intros red1 red2.
-    induction red1.
-    
-  Lemma red_p_det (c c1 c2 : cmd) (st st1 st2 : stack) (ph ph1 ph2 : pheap) :
-    is_pheap ph -> is_pheap ph1 -> is_pheap ph2 ->
-    c / (st, ph) ==>p c1 / (st1, ph1) ->
-    c / (st, ph) ==>p c2 / (st2, ph2) ->
-    c1 = c2 /\ st1 = st2 /\ ph1 = ph2.
-  Proof.
-    intros isp isp1 isp2 red1 red2;
-    inversion red1.
-  
+    induction [c2 st2 red2]red1; intros c2' st2 red2; try (inversion red2; subst; split; congruence).
+    - inversion red2; subst; eauto.
+      inversion R.
+    - inversion red2; subst.
+      + inversion red1.
+      + apply IHred1 in R; destruct R; subst; split; congruence.
+  Qed.
+
   Fixpoint accesses (c : cmd) (s : stack) := 
     match c with
-      | Cskip => nil
-      | x ::= e => nil
-      | x ::= [e] => edenot e s :: nil
-      | [e] ::= e' => edenot e s :: nil
+      | Cskip => None
+      | x ::= e => None
+      | x ::= [e] => Some (edenot e s)
+      | [e] ::= e' => Some (edenot e s)
       | c1 ;; c2 => accesses c1 s
-      | (Cif b c1 c2) => nil
-      | (Cwhile b c) => nil
-      | (Cbarrier _) => nil
+      | (Cif b c1 c2) => None
+      | (Cwhile b c) => None
+      | (Cbarrier _) => None
     end.
 
   Fixpoint writes (c : cmd) (s : stack) :=
     match c with
-      | Cskip => nil
-      | (x ::= e) => nil
-      | (x ::= [e]) => nil
-      | ([e] ::= e') => edenot e s :: nil
+      | Cskip => None
+      | (x ::= e) => None
+      | (x ::= [e]) => None
+      | ([e] ::= e') => Some (edenot e s)
       | (c1 ;; c2) => writes c1 s
-      | (Cif b c1 c2) => nil
-      | (Cwhile b c) => nil
-      | Cbarrier j => nil
+      | (Cif b c1 c2) => None
+      | (Cwhile b c) => None
+      | Cbarrier j => None
     end.
   
   Inductive aborts : cmd -> state -> Prop := 
@@ -494,8 +500,8 @@ Module Language.
                        (Cbarrier j) / ss || Some (j, Cskip) / ss
       where " c '/' s '||' c' '/' s'" := (eval c s c' s').
     
-    Lemma red1_eval (x y : (cmd * state)) (st : state) : 
-      red x y -> (fst y) / (snd y) || None / st -> fst x / snd x || None / st.
+    Lemma red1_eval (c1 c2 : cmd) (st1 st2 : state) (st : state) : 
+      c1 / st1 ==>s c2 / st2 -> c2 / st2 || None / st -> c1 / st1 || None / st.
     Proof.
       move=> H IH.
       induction [st IH]H; ins; try do 10 (econstructor; eauto).
@@ -563,6 +569,7 @@ Module Language.
       - move=>->; simpl in *.
         assert ((c', st') = (c', st')) as IH by eauto; apply IHhs in IH; clear IHhs; simpl in *.
         clear hs hwait c' c st.
+        unfold red_tup in H;
         induction [c'' IH]H; ins; try do 5 (econstructor; eauto).
         + inversion IH; subst.
           * apply eval_Seq1. 
@@ -575,4 +582,208 @@ Module Language.
         + inversion IH.
     Qed.
   End BigStep.
+
+  Definition kstate := (list (cmd * stack) * heap)%type.
+
+  Module PLang.
+    Definition pstate := (stack * pheap)%type.
+  
+    Definition access_ok (c : cmd) (s : stack) (h : pheap) :=
+      match accesses c s with
+        | None => True
+        | Some v => exists x, this h v = Some x
+      end.
+
+    Definition write_ok (c : cmd) (s : stack) (h : pheap) :=
+      match writes c s with
+        | None => True
+        | Some v => exists x, this h v = Some (full_p, x)
+      end.
+
+    Inductive red_p: cmd -> pstate -> cmd -> pstate -> Prop :=
+      redp_ster : forall (c1 c2 : cmd) (st1 st2 : state) (pst1 pst2 : pstate) (s1 s2 : stack)
+                         (ph1 ph2 phF : pheap) (h1 h2 : heap),
+        st1 = (s1, h1) -> st2 = (s2, h2) ->
+        pst1 = (s1, ph1) -> pst2 = (s2, ph2) ->
+        access_ok c1 s1 ph1 ->
+        write_ok c1 s1 ph1 ->
+        pdisj ph1 phF -> ptoheap (phplus ph1 phF) h1 ->
+        c1 / st1 ==>s c2 / st2 ->
+        pdisj ph2 phF -> ptoheap (phplus ph2 phF) h2 ->
+        red_p c1 pst1 c2 pst2.
+    Notation "c '/' st  '==>p'  c' '/' st' " := 
+      (red_p c st c' st') (at level 40, st at level 39, c' at level 39).
+
+    Hint Resolve pdisjC.
+    Lemma Q1 (q1 q2 q : Qc) : q1 + q2 = q -> q1 = q - q2.
+    Proof. intros H; rewrite <-H; ring. Qed.
+    Hint Rewrite Q1.
+
+    Lemma Q2 (q1 q2 q : Qc) : q1 + q2 = q -> q2 = q - q1.
+    Proof. intros H; rewrite <-H; ring. Qed.
+    Hint Rewrite Q2.
+
+    Lemma phplus_cancel_toheap (ph1 ph2 phF : pheap) (h : heap):
+      pdisj ph1 phF -> pdisj ph2 phF ->
+      ptoheap (phplus ph1 phF) h -> ptoheap (phplus ph2 phF) h -> ph1 = ph2.
+    Proof.
+      intros dis1 id2 to1 to2.
+      pose proof (ptoD to1 to2).
+      eapply padd_cancel2; eauto.
+    Qed.
+
+    Lemma padd_upd_cancel (ph1 ph2 phF : pheap) (h : heap) (x v v': Z) :
+      pdisj ph1 phF -> pdisj ph2 phF -> ptoheap (phplus ph1 phF) h ->
+      this ph1 x = Some (full_p, v') -> ptoheap (phplus ph2 phF) (upd h x (Some v)) -> 
+      this ph2 = ph_upd ph1 x v.
+    Proof.
+      intros pd1 pd2 toh1 have1 toh2; extensionality y; unfold ph_upd.
+      destruct ph1 as [ph1 h1], ph2 as [ph2 h2], phF as [phF hF]; simpl in *.
+      destruct (Z.eq_dec x y).
+      - rewrite <-e; clear e y.
+        unfold is_pheap, pdisj, ptoheap, upd, phplus in *;
+          repeat (match goal with [H : forall _ : Z, _ |- _] => specialize (H x) end).
+        destruct (Z.eq_dec x x); try tauto.
+        rewrite have1 in *.
+        destruct (phF x) as [[pF vF]|]; des.
+        + apply Qcle_minus_iff in pd3.
+          cutrewrite (1 + -(full_p + pF) = -pF) in pd3; [|unfold full_p; field].
+          apply Qcopp_le_compat in pd3; ring_simplify in pd3.
+          apply Qcle_not_lt in pd3; tauto.
+        + destruct (ph2 x) as [[p2 v2]|]; try congruence.
+          des; congruence.
+      - unfold is_pheap, pdisj, ptoheap, upd, phplus in *;
+        repeat (match goal with [H : forall _ : Z, _ |- _] => specialize (H y) end).
+        destruct (Z.eq_dec y x); [symmetry in e; tauto |].
+        destruct (ph1 y) as [[? ?]|], (phF y) as [[? ?]|], (ph2 y) as [[? ?]|]; des; 
+        try congruence.
+        apply Q1 in toh1; apply Q1 in toh2.
+        destruct (h y) as [? | ]; inversion toh0; inversion toh3; congruence.
+        rewrite toh2 in toh1.
+        assert (q + full_p - full_p = full_p - full_p) by (rewrite toh1; ring).
+        ring_simplify in H; rewrite H in h1; inversion h1.
+        rewrite toh1 in toh2.
+        assert (q0 + full_p - full_p = full_p - full_p) by (rewrite toh2; ring).
+        ring_simplify in H; rewrite H in h2; inversion h2.
+    Qed.
+
+    Lemma red_p_det (c c1 c2 : cmd) (st st1 st2 : pstate) :
+      c / st ==>p c1 / st1 ->
+      c / st ==>p c2 / st2 ->
+      c1 = c2 /\ st1 = st2.
+    Proof.
+      intros red1 red2.
+      destruct red1 as
+          [c1 c1' st1 st1' pst1 pst1' s1 s1' ph1 ph1' phF1 h1 h1' eq1 eq1' 
+              peq1 peq1' aok1 wok1 dis1 to1 red1 dis1' to1'].
+      destruct red2 as
+          [c2 c2' st2 st2' pst2 pst2' s2 s2' ph2 ph2' phF2 h2 h2' eq2 eq2' 
+              peq2 peq2' aok2 wok2 dis2 to2 red2 dis2' to2'].
+      induction [c2' red2]red1; intros c2' red2; 
+      try (inversion red2; subst; 
+           repeat (match goal with [H : (_, _) = (_, _) |- _ ] => inversion H; subst; clear H end);
+           simpl in *; try congruence;
+           assert (ph1' = ph2) by (eapply phplus_cancel_toheap; eauto);
+           assert (ph2' = ph2) by (eapply phplus_cancel_toheap; eauto);
+           split; congruence).
+      - inversion red2; subst.
+        + repeat (match goal with [H : (_, _) = (_, _) |- _ ] => inversion H; subst; clear H end).
+          assert (ph1' = ph2) by (eapply phplus_cancel_toheap; eauto).
+          assert (ph2' = ph2) by (eapply phplus_cancel_toheap; eauto).
+          split; congruence.
+        + inversion R.
+      - inversion red2; subst. 
+        + inversion red1.
+        + unfold access_ok, write_ok in *; simpl in *. 
+          pose proof (IHred1 eq_refl eq_refl aok1 wok1 aok2 wok2 c1'0 R) as H; 
+            destruct H as [He1 He2].
+          split; [subst; eauto | eauto].
+      - inversion red2; subst;
+        repeat (match goal with [H : (_, _) = (_, _) |- _ ] => inversion H; subst; clear H end).
+        unfold access_ok in *; simpl in *.
+        remember (edenot e s0) as vad.
+        assert (ph1' = ph2) by (eapply phplus_cancel_toheap; eauto).
+        assert (ph2' = ph2) by (eapply phplus_cancel_toheap; eauto).
+        cutrewrite (v = v0); [split; congruence |].
+        assert (Some v0 = Some v) as Heq; [ rewrite <- RD0, <-RD | 
+                                            rewrite <-RD0, <-RD in Heq; congruence].
+        clear Heqvad; subst.
+        destruct aok1 as [[q va] Hv].
+        unfold pdisj, ptoheap in *.
+        repeat (match goal with [H : forall _ : Z, _ |- _] => specialize (H vad) end).
+        unfold phplus in *.
+        rewrite Hv in *.
+        destruct (this phF1 vad) as [[? ?] | ], (this phF2 vad) as [[? ?] | ]; des; try congruence.
+      - inversion red2; subst.
+        split; eauto.
+        assert (s1' = s2') by congruence; subst.
+        assert (ph1' = ph2'); [| subst; eauto].
+        inversion EQ3; inversion EQ0; inversion peq2; inversion EQ2; inversion EQ1. 
+        subst. rewrite H8 in *.
+        unfold write_ok in *; simpl in *.
+        destruct wok1 as [v1' H1], wok2 as [v2' H2].
+        remember (edenot e1 s) as addr. clear Heqaddr.
+        remember (edenot e2 s) as v. clear Heqv.
+        assert (this ph1' = ph_upd ph2 addr v) by eapply (padd_upd_cancel dis1 dis1' to1 H1 to1').
+        assert (this ph2' = ph_upd ph2 addr v) by eapply (padd_upd_cancel dis2 dis2' to2 H2 to2').
+        destruct ph1' as [ph1' h1], ph2' as [ph2' h2]; simpl in *; subst.
+        assert (h1 = h2) by apply proof_irrelevance; congruence.
+    Qed.
+
+    Section Typing.
+      Inductive type := Hi | Lo.
+      Definition join (t1 t2 : type) :=
+        match (t1, t2) with
+          | (Hi, _) | (_, Hi) => Hi
+          | (Lo, Lo) => Lo
+        end.
+      
+      Definition le_type (t1 t2 : type) : bool :=
+        match (t1, t2) with
+          | (Lo, _) | (_, Hi) => true
+          | (Hi, Lo) => false
+        end.
+
+      Definition env := var -> type.
+      Inductive typing_exp : env -> exp -> type -> Prop := 
+      | ty_var : forall (g : env) (v : var) (ty : type), g v = ty -> typing_exp g (Evar v) ty
+      | ty_num : forall (g : env) (n : Z) (ty : type), typing_exp g (Enum n) ty
+      | ty_plus : forall (g : env) (e1 e2 : exp) (ty1 ty2 : type), 
+                    typing_exp g e1 ty1 -> typing_exp g e2 ty2 ->
+                    typing_exp g (Eplus e1 e2) (join ty1 ty2).
+
+      Inductive typing_bexp : env -> bexp -> type -> Prop := 
+      | ty_eq : forall (g : env) (e1 e2 : exp) (ty1 ty2 : type), 
+                  typing_exp g e1 ty1 -> typing_exp g e2 ty2 ->
+                  typing_bexp g (Beq e1 e2) (join ty1 ty2)
+      | ty_and : forall (g : env) (b1 b2 : bexp) (ty1 ty2 : type), 
+                  typing_bexp g b1 ty1 -> typing_bexp g b2 ty2 ->
+                  typing_bexp g (Band b1 b2) (join ty1 ty2)
+      | ty_not : forall (g : env) (b : bexp) (ty : type), 
+                   typing_bexp g b ty -> typing_bexp g (Bnot b) ty.
+
+      Inductive typing_cmd : env -> cmd -> type -> Prop :=
+      | ty_skip : forall (g : env) (pc : type), typing_cmd g Cskip pc
+      | ty_assign : forall (g : env) (v : var) (e : exp) (pc ty : type),
+                      typing_exp g e ty -> le_type (join ty pc) (g v) = true ->
+                      typing_cmd g (v ::= e) pc
+      | ty_read : forall (g : env) (v : var) (e : exp) (pc ty : type),
+                    typing_exp g e ty -> le_type (join ty pc) (g v) = true ->
+                    typing_cmd g (v ::= [e]) pc
+      | ty_write : forall (g : env) (e1 e2 : exp) (pc : type),
+                     typing_cmd g ([e1] ::= e2) pc
+      | ty_seq : forall (g : env) (c1 c2 : cmd) (pc : type),
+                   typing_cmd g c1 pc -> typing_cmd g c2 pc ->
+                   typing_cmd g (c1 ;; c2) pc
+      | ty_if : forall (g : env) (b : bexp) (c1 c2 : cmd) (pc ty : type),
+                  typing_bexp g b ty ->
+                  typing_cmd g c1 (join pc ty) -> typing_cmd g c2 (join pc ty) ->
+                  typing_cmd g (Cif b c1 c2) pc
+      | ty_while : forall (g : env) (b : bexp) (c : cmd) (pc ty : type),
+                     typing_bexp g b ty ->
+                     typing_cmd g c (join pc ty) -> typing_cmd g (Cwhile b c) pc
+      | ty_barrier : forall (g : env) (j : nat), typing_cmd g (Cbarrier j) Lo.
+
+      
+
 End Language.
